Some clean up and refactoring for relcom example

aneris/examples/reliable_communication/resources/session_escrow.v
@@ -1,13 +1,13 @@
+From iris.bi Require Import updates.
 From iris.algebra Require Import agree gmap auth excl numbers frac_auth csum.
 From iris.algebra.lib Require Import excl_auth mono_nat.
 From iris.base_logic.lib Require Import invariants mono_nat.
 From iris.proofmode Require Import tactics.
 From aneris.aneris_lang Require Import resources.
-From aneris.examples.reliable_communication.resources Require Export mono_list.
-From actris.channel Require Import proto.
 From aneris.aneris_lang.program_logic Require Import aneris_weakestpre step_update.
-From iris.bi Require Import updates.
 From aneris.aneris_lang.state_interp Require Import state_interp_def.
+From aneris.examples.reliable_communication.resources
+     Require Export mono_list step_proto.
 
 Set Default Proof Using "Type".
 
@@ -57,14 +57,6 @@ Section iProto_sessions.
   Context `{!session_escrowG Σ A, !anerisG Mdl Σ}.
   Context (N : namespace).
 
-  Parameter γc : proto_name.
-  Parameter γTl : gname.
-  Parameter γTr : gname.
-  Parameter γsl : gname.
-  Parameter γrl : gname.
-  Parameter γsr : gname.
-  Parameter γrr : gname.
-
   Definition auth_list (χ : session_escrow_name) (s : side) (xs : list A) :=
     own (side_elim s (χ.(session_escrow_Tl_name)) (χ.(session_escrow_Tr_name)))
         (●ML (xs : list (leibnizO A))).
@@ -90,60 +82,46 @@ Definition auth_auth_sent (χ : session_escrow_name) (s : side) (n : nat) : iPro
   Definition Ses_inv (χ : session_escrow_name) : iProp Σ :=
     ∃ (Tl Tr : list A) (nl nr : nat),
       ⌜nr ≤ length Tl⌝ ∗ ⌜nl ≤ length Tr⌝ ∗
-      iProto_ctx χ.(session_escrow_proto_name) (drop nr Tl) (drop nl Tr) ∗
+      iProto_step_ctx χ.(session_escrow_proto_name) (drop nr Tl) (drop nl Tr) ∗
       auth_list χ Left Tl ∗ auth_list χ Right Tr ∗
       auth_auth_sent χ Left (length Tl) ∗ auth_auth_recv χ Left nl ∗
-      auth_auth_sent χ Right (length Tr) ∗ auth_auth_recv χ Right nr ∗
-      steps_lb (length Tl) ∗ steps_lb (length Tr).
+      auth_auth_sent χ Right (length Tr) ∗ auth_auth_recv χ Right nr.
 
   Definition Ses (χ : session_escrow_name) : iProp Σ :=
     inv N (Ses_inv χ).
 
-  Definition ses_own (χ : session_escrow_name) (s : side) (n m : nat) (p : iProto Σ A) : iProp Σ :=
+  Definition ses_own_def (χ : session_escrow_name) (s : side) (n m : nat) (p : iProto Σ A) : iProp Σ :=
     Ses χ ∗
     iProto_own χ.(session_escrow_proto_name) s p ∗
     auth_frag_sent χ s n ∗ auth_frag_recv χ s m.
+  Definition ses_own_aux : seal (ses_own_def). by eexists. Qed.
+  Definition ses_own := ses_own_aux.(unseal).
+  Definition ses_own_eq : @ses_own = @ses_own_def := ses_own_aux.(seal_eq).
+  Global Instance: Params (@ses_own) 5 := {}.
 
   Global Instance ses_own_contractive χ s n m : Contractive (ses_own χ s n m).
-  Proof. solve_contractive. Qed.
+  Proof. rewrite ses_own_eq. solve_contractive. Qed.
   Global Instance ses_own_ne χ s n m : NonExpansive (ses_own χ s n m).
-  Proof. solve_proper. Qed.
+  Proof. rewrite ses_own_eq. solve_proper. Qed.
   Global Instance ses_own_proper χ s n m : Proper ((≡) ==> (≡)) (ses_own χ s n m).
-  Proof. solve_proper. Qed.
+  Proof. rewrite ses_own_eq. solve_proper. Qed.
 
-  Definition ses_idx (χ : session_escrow_name) (s : side) (n : nat) (x : A) :=
+  Definition ses_idx_def (χ : session_escrow_name) (s : side) (n : nat) (x : A) :=
     frag_list χ s n x.
+  Definition ses_idx_aux : seal (ses_idx_def). by eexists. Qed.
+  Definition ses_idx := ses_idx_aux.(unseal).
+  Definition ses_idx_eq : @ses_idx = @ses_idx_def := ses_idx_aux.(seal_eq).
+  Global Instance: Params (@ses_idx) 4 := {}.
 
   Global Instance ses_idx_contractive χ s n v : Persistent (ses_idx χ s n v).
-  Proof. apply _. Qed.
+  Proof. rewrite ses_idx_eq. apply _. Qed.
 
   Lemma ses_own_le χ s n m p1 p2 :
     ses_own χ s n m p1 -∗ ▷ (p1 ⊑ p2) -∗ ses_own χ s n m p2.
   Proof.
+    rewrite ses_own_eq.
     iIntros "(Hinv & Hp & H) Hle".
     iDestruct (iProto_own_le with "Hp Hle") as "Hp". by iFrame.
-  Qed.
-
-  Lemma Ses_init E p :
-    ⊢ steps_lb 0 ={E}=∗ ∃ χ, Ses χ ∗ ses_own χ Left 0 0 p ∗
-                   ses_own χ Right 0 0 (iProto_dual p).
-  Proof.
-    iIntros "#Hsteps".
-    iMod (iProto_init p) as (γc) "(Hctx & Hpl & Hpr)".
-    iMod (own_alloc (●ML [])) as (γl) "Hl"; [apply mono_list_auth_valid|].
-    iMod (own_alloc (●ML [])) as (γr) "Hr"; [apply mono_list_auth_valid|].
-    iMod (own_alloc (●E 0%nat ⋅ ◯E 0%nat)) as (γsl) "[HslA HslF]"; [apply excl_auth_valid|].
-    iMod (own_alloc (●E 0%nat ⋅ ◯E 0%nat)) as (γrl) "[HrlA HrlF]"; [apply excl_auth_valid|].
-    iMod (own_alloc (●E 0%nat ⋅ ◯E 0%nat)) as (γsr) "[HsrA HsrF]"; [apply excl_auth_valid|].
-    iMod (own_alloc (●E 0%nat ⋅ ◯E 0%nat)) as (γrr) "[HrrA HrrF]"; [apply excl_auth_valid|].
-    set (χ := SessionEscrowName γc γl γr γsl γrl γsr γrr).
-    iMod (inv_alloc N E (Ses_inv χ) with "[Hctx Hl Hr HslA HrlA HsrA HrrA]")
-      as "#H".
-    { iIntros "!>". iExists [], [], 0%nat, 0%nat. iFrame "#∗".
-      iSplit; iPureIntro; lia. }
-    iModIntro.
-    iExists χ.
-    iFrame "#∗".
   Qed.
 
   (* Have this lemma to make it consistent with the others of the ghost theory. *)
@@ -153,7 +131,8 @@ Definition auth_auth_sent (χ : session_escrow_name) (s : side) (n : nat) : iPro
   Proof.
     iApply step_get_impl; [iApply step_get_lb_get|].
     iIntros "#Hsteps".
-    iMod (iProto_init p) as (γc) "(Hctx & Hpl & Hpr)".
+    iApply step_get_impl; [iApply (iProto_step_init E p)|].
+    iDestruct 1 as (γc) "(Hctx & Hpl & Hpr)".
     iMod (own_alloc (●ML [])) as (γl) "Hl"; [apply mono_list_auth_valid|].
     iMod (own_alloc (●ML [])) as (γr) "Hr"; [apply mono_list_auth_valid|].
     iMod (own_alloc (●E 0%nat ⋅ ◯E 0%nat)) as (γsl) "[HslA HslF]"; [apply excl_auth_valid|].
@@ -163,12 +142,13 @@ Definition auth_auth_sent (χ : session_escrow_name) (s : side) (n : nat) : iPro
     set (χ := SessionEscrowName γc γl γr γsl γrl γsr γrr).
     iMod (inv_alloc N E (Ses_inv χ) with "[Hctx Hl Hr HslA HrlA HsrA HrrA]")
       as "#H".
-    { iIntros "!>". iExists [], [], 0%nat, 0%nat. iFrame "#∗".
+    { iIntros "!>". iExists [], [], 0%nat, 0%nat. iFrame.
       iSplit; iPureIntro; lia. }
     iIntros (n) "Hauth". iApply fupd_mask_intro; [set_solver|].
     iIntros "Hclose". iFrame. iMod "Hclose".
     iModIntro.
     iExists χ.
+    rewrite !ses_own_eq.
     iFrame "#∗".
   Qed.
 
@@ -177,87 +157,67 @@ Definition auth_auth_sent (χ : session_escrow_name) (s : side) (n : nat) : iPro
     ses_own χ s n m (<!> pm)%proto -∗ iMsg_car pm v (Next p) -∗
     |~{E}~> (ses_own χ s (S n) m p ∗ ses_idx χ s n v).
   Proof.
+    rewrite ses_own_eq ses_idx_eq.
     iIntros (HE) "[#HI (Hp&HsF&HrF)] Hpm".
     iApply step_update_open.
     iInv N as "H" "Hclose".
     iDestruct "H" as (Tl Tr nl nr)
-                       "(>%Hle&>%Hle2&Hctx&>HTl&>HTr&
-                       >Hsl&>Hrl&>Hsr&>Hrr&#>HTllb&#>HTrlb)".
+                       "(>%Hle&>%Hle2&Hctx&>HTl&>HTr&>Hsl&>Hrl&>Hsr&>Hrr)".
     destruct s.
-    -  iDestruct (step_update_lb_step with "HTrlb [Hctx Hp Hpm]") as "Hctx".
-       { simpl. iIntros "!>!>".
-         iApply step_fupdN_intro; [done|].
-         iMod (iProto_send_l with "Hctx Hp Hpm") as "H". iModIntro.
-         iApply (bi.laterN_le (length (drop nl Tr)) with "[H]");
-           [rewrite drop_length; lia|].
-         iIntros "!>"=> /=. iExact "H". }
-       iDestruct (step_update_lb_update with "HTllb") as "HTllb'".
-       iDestruct (step_update_comm (E∖↑N) ∅ with "Hctx HTllb'") as "Hstep";
-         [set_solver|].
-       rewrite union_empty_r_L.
-       iModIntro.
-       iApply (step_update_mono with "Hstep"); [set_solver|]; iIntros "Hstep".
-       iDestruct "Hstep" as "[[Hctx Hp] #HTllb'']".
-       iModIntro.
-       iDestruct (own_valid_2 with "Hsl HsF") as %Hvalid1%excl_auth_agree_L.
-       iDestruct (own_valid_2 with "Hrl HrF") as %Hvalid2%excl_auth_agree_L.
-       iMod (own_update_2 _ _ _ (●E (S (length Tl)) ⋅ ◯E (S (length Tl)))
-              with "Hsl HsF") as "[Hsl HsF]"; [by apply excl_auth_update|].
-       iMod (own_update _ _ (●ML ((Tl ++ [v]):list (leibnizO A)))
-              with "HTl") as "HTl".
-       { apply mono_list_update. by apply prefix_app_r. }
-       rewrite mono_list_auth_lb_op.
-       iDestruct "HTl" as "[HTl HTl']".
-       iAssert (frag_list χ Left n v) with "[HTl']" as "Hidx".
-       { iExists _. iFrame. iPureIntro. rewrite -Hvalid1.
-         rewrite lookup_app_r; [|lia]. rewrite minus_diag. done. }
-       rewrite Hvalid1.
-       iFrame "#∗".
-       iApply "Hclose".
-       iIntros "!>".
-       rewrite -drop_app_le; [|lia].
-       iExists (Tl ++ [v]), Tr, nl, nr.
-       rewrite app_length. rewrite Hvalid1. simpl.
-       replace (S n) with (n + 1)%nat by lia.
-       iFrame "#∗".
-       iSplit; iPureIntro; lia.
-    -  iDestruct (step_update_lb_step with "HTllb [Hctx Hp Hpm]") as "Hctx".
-       { simpl. iIntros "!>!>".
-         iApply step_fupdN_intro; [done|].
-         iMod (iProto_send_r with "Hctx Hp Hpm") as "H". iModIntro.
-         iApply (bi.laterN_le (length (drop nr Tl)) with "[H]");
-           [rewrite drop_length; lia|].
-         iIntros "!>"=> /=. iExact "H". }
-       iDestruct (step_update_lb_update with "HTrlb") as "HTrlb'".
-       iDestruct (step_update_comm (E∖↑N) ∅ with "Hctx HTrlb'") as "Hstep";
-         [set_solver|].
-       rewrite union_empty_r_L.
-       iModIntro.
-       iApply (step_update_mono with "Hstep"); [set_solver|]; iIntros "Hstep".
-       iDestruct "Hstep" as "[[Hctx Hp] #HTrlb'']".
-       iModIntro.
-       iDestruct (own_valid_2 with "Hsr HsF") as %Hvalid1%excl_auth_agree_L.
-       iDestruct (own_valid_2 with "Hrr HrF") as %Hvalid2%excl_auth_agree_L.
-       iMod (own_update_2 _ _ _ (●E (S (length Tr)) ⋅ ◯E (S (length Tr)))
-              with "Hsr HsF") as "[Hs HsF]"; [by apply excl_auth_update|].
-       iMod (own_update _ _ (●ML ((Tr ++ [v]):list (leibnizO A)))
-              with "HTr") as "HTr".
-       { apply mono_list_update. by apply prefix_app_r. }
-       rewrite mono_list_auth_lb_op.
-       iDestruct "HTr" as "[HTr HTr']".
-       iAssert (frag_list χ Right n v) with "[HTr']" as "Hidx".
-       { iExists _. iFrame. iPureIntro. rewrite -Hvalid1.
-         rewrite lookup_app_r; [|lia]. rewrite minus_diag. done. }
-       rewrite Hvalid1.
-       iFrame "#∗".
-       iApply "Hclose".
-       iIntros "!>".
-       rewrite -drop_app_le; [|lia].
-       iExists Tl, (Tr ++ [v]), nl, nr.
-       rewrite app_length. rewrite Hvalid1. simpl.
-       replace (S n) with (n + 1)%nat by lia.
-       iFrame "#∗".
-       iSplit; iPureIntro; lia.
+    - iApply (step_update_impl with "[Hctx Hp Hpm]");
+        [iApply (iProto_step_send_l with "Hctx Hp Hpm")|].
+      iModIntro.
+      iApply step_update_intro; [set_solver|].
+      iIntros "[Hctx Hp]".
+      iDestruct (own_valid_2 with "Hsl HsF") as %Hvalid1%excl_auth_agree_L.
+      iDestruct (own_valid_2 with "Hrl HrF") as %Hvalid2%excl_auth_agree_L.
+      iMod (own_update_2 _ _ _ (●E (S (length Tl)) ⋅ ◯E (S (length Tl)))
+             with "Hsl HsF") as "[Hsl HsF]"; [by apply excl_auth_update|].
+      iMod (own_update _ _ (●ML ((Tl ++ [v]):list (leibnizO A)))
+             with "HTl") as "HTl".
+      { apply mono_list_update. by apply prefix_app_r. }
+      rewrite mono_list_auth_lb_op.
+      iDestruct "HTl" as "[HTl HTl']".
+      iAssert (frag_list χ Left n v) with "[HTl']" as "Hidx".
+      { iExists _. iFrame. iPureIntro. rewrite -Hvalid1.
+        rewrite lookup_app_r; [|lia]. rewrite minus_diag. done. }
+      rewrite Hvalid1.
+      iFrame "#∗".
+      iApply "Hclose".
+      iIntros "!>".
+      rewrite -drop_app_le; [|lia].
+      iExists (Tl ++ [v]), Tr, nl, nr.
+      rewrite app_length. rewrite Hvalid1. simpl.
+      replace (S n) with (n + 1)%nat by lia.
+      iFrame.
+      iSplit; iPureIntro; lia.
+    - iApply (step_update_impl with "[Hctx Hp Hpm]");
+        [iApply (iProto_step_send_r with "Hctx Hp Hpm")|].
+      iModIntro.
+      iApply step_update_intro; [set_solver|].
+      iIntros "[Hctx Hp]".
+      iDestruct (own_valid_2 with "Hsr HsF") as %Hvalid1%excl_auth_agree_L.
+      iDestruct (own_valid_2 with "Hrr HrF") as %Hvalid2%excl_auth_agree_L.
+      iMod (own_update_2 _ _ _ (●E (S (length Tr)) ⋅ ◯E (S (length Tr)))
+             with "Hsr HsF") as "[Hs HsF]"; [by apply excl_auth_update|].
+      iMod (own_update _ _ (●ML ((Tr ++ [v]):list (leibnizO A)))
+             with "HTr") as "HTr".
+      { apply mono_list_update. by apply prefix_app_r. }
+      rewrite mono_list_auth_lb_op.
+      iDestruct "HTr" as "[HTr HTr']".
+      iAssert (frag_list χ Right n v) with "[HTr']" as "Hidx".
+      { iExists _. iFrame. iPureIntro. rewrite -Hvalid1.
+        rewrite lookup_app_r; [|lia]. rewrite minus_diag. done. }
+      rewrite Hvalid1.
+      iFrame "#∗".
+      iApply "Hclose".
+      iIntros "!>".
+      rewrite -drop_app_le; [|lia].
+      iExists Tl, (Tr ++ [v]), nl, nr.
+      rewrite app_length. rewrite Hvalid1. simpl.
+      replace (S n) with (n + 1)%nat by lia.
+      iFrame "#∗".
+      iSplit; iPureIntro; lia.
   Qed.
 
   Lemma step_update_recv_l χ E n m pm v :
@@ -265,12 +225,12 @@ Definition auth_auth_sent (χ : session_escrow_name) (s : side) (n : nat) : iPro
     ses_own χ Left n m (<?> pm)%proto -∗ ses_idx χ Right m v -∗
     |~{E}~> ∃ p, ses_own χ Left n (S m) p ∗ iMsg_car pm v (Next p).
   Proof.
+    rewrite !ses_own_eq !ses_idx_eq.
     iIntros (HE) "[#HI (Hp&HslF&HrlF)] Hidx".
     iApply step_update_open.
     iInv N as "H" "Hclose".
     iDestruct "H" as (Tl Tr nl nr)
-                       "(>%Hle&>%Hle2&Hctx&>HTl&>HTr&
-                         >Hsl&>Hrl&>Hsr&>Hrr&#>HTllb&#>HTrlb)".
+                       "(>%Hle&>%Hle2&Hctx&>HTl&>HTr&>Hsl&>Hrl&>Hsr&>Hrr)".
     iDestruct (own_valid_2 with "Hrl HrlF") as %Hvalid%excl_auth_agree_L.
     rewrite Hvalid.
     iDestruct "Hidx" as (Tr') "[%Hlookup HTr']".
@@ -281,21 +241,15 @@ Definition auth_auth_sent (χ : session_escrow_name) (s : side) (n : nat) : iPro
     rewrite drop_app_le; last first.
     { by apply Nat.lt_le_incl. }
     rewrite (drop_S Tr' v m); [|done]=> /=.
-    iApply step_update_lb_step; [iApply "HTrlb"|]=> /=.
-    assert (1 ≤ length Tr') by lia.
-    iFrame.
-    iIntros "!>!>!>".
-    iMod (iProto_recv_l with "Hctx Hp") as (p) "(Hctx & Hp &HP)".
+    iModIntro.
+    iApply (step_update_impl with "[Hctx Hp]");
+      [iApply (iProto_step_recv_l with "Hctx Hp")|].
+    iApply step_update_intro; [set_solver|].
+    iDestruct 1 as (p) "(Hctx & Hp &HP)".
     iMod (own_update_2 _ _ _ (●E (S m) ⋅ ◯E (S m))
            with "Hrl HrlF") as "[Hrl HrlF]"; [by apply excl_auth_update|].
-    iModIntro.
-    simpl.
     destruct Tr' as [|r Tr']; [done|]=> /=.
-    iIntros "!>!>!>".
-    iApply step_fupdN_intro; [done|].
-    iIntros "!>".
-    iFrame.
-    iMod ("Hclose" with "[-Hp HP]") as "_".
+    iMod ("Hclose" with "[-Hp HP HslF HrlF]") as "_".
     { iNext. iExists Tl,((r::Tr')++Tr''),(S m),nr. iFrame "#∗".
       rewrite drop_app_le; last first.
       { apply lt_n_Sm_le, le_n_S. done. }
@@ -314,12 +268,12 @@ Definition auth_auth_sent (χ : session_escrow_name) (s : side) (n : nat) : iPro
     ses_own χ Right n m (<?> pm)%proto -∗ ses_idx χ Left m v -∗
     |~{E}~> ∃ p, ses_own χ Right n (S m) p ∗ iMsg_car pm v (Next p).
   Proof.
+    rewrite !ses_own_eq !ses_idx_eq.
     iIntros (HE) "[#HI (Hp&HsrF&HrrF)] Hidx".
     iApply step_update_open.
     iInv N as "H" "Hclose".
     iDestruct "H" as (Tl Tr nl nr)
-                       "(>%Hle&>%Hle2&Hctx&>HTl&>HTr&
-                         >Hsl&>Hrl&>Hsr&>Hrr&#>HTllb&#>HTrlb)".
+                       "(>%Hle&>%Hle2&Hctx&>HTl&>HTr&>Hsl&>Hrl&>Hsr&>Hrr)".
     iDestruct (own_valid_2 with "Hrr HrrF") as %Hvalid%excl_auth_agree_L.
     rewrite Hvalid.
     iDestruct "Hidx" as (Tl') "[%Hlookup HTl']".
@@ -330,21 +284,16 @@ Definition auth_auth_sent (χ : session_escrow_name) (s : side) (n : nat) : iPro
     rewrite drop_app_le; last first.
     { by apply Nat.lt_le_incl. }
     rewrite (drop_S Tl' v m); [|done]=> /=.
-    iApply step_update_lb_step; [iApply "HTllb"|]=> /=.
-    assert (1 ≤ length Tl') by lia.
-    iFrame.
-    iIntros "!>!>!>".
-    iMod (iProto_recv_r with "Hctx Hp") as (p) "(Hctx & Hp &HP)".
+    iModIntro.
+    iApply (step_update_impl with "[Hctx Hp]");
+      [iApply (iProto_step_recv_r with "Hctx Hp")|].
+    iApply step_update_intro; [set_solver|].
+    iDestruct 1 as (p) "(Hctx & Hp &HP)".
     iMod (own_update_2 _ _ _ (●E (S m) ⋅ ◯E (S m))
            with "Hrr HrrF") as "[Hrr HrrF]"; [by apply excl_auth_update|].
-    iModIntro.
     simpl.
     destruct Tl' as [|l Tl']; [done|]=> /=.
-    iIntros "!>!>!>".
-    iApply step_fupdN_intro; [done|].
-    iIntros "!>".
-    iFrame.
-    iMod ("Hclose" with "[-Hp HP]") as "_".
+    iMod ("Hclose" with "[-Hp HP HsrF HrrF]") as "_".
     { iNext. iExists ((l::Tl')++Tl''),Tr,nl,(S m). iFrame "#∗".
       rewrite drop_app_le; last first.
       { apply lt_n_Sm_le, le_n_S. done. }
